code/ecdsap256sha2/Hacl.Impl.P256.Compression.fsti
@@ -18,15 +18,26 @@ open Spec.P256.MontgomeryMultiplication
 let notCompressedForm = lbuffer uint8 (size 65)
 let compressedForm = lbuffer uint8 (size 33)
 
-(* the name makes a lot of sense, doesnot it? *)
-
 (* the function is to decode publickey, so NOT SCA resistant *)
 
 (*void uECC_decompress(const uint8_t *compressed, uint8_t *public_key, uECC_Curve curve)  *)
 
 val decompressionNotCompressedForm: b: notCompressedForm -> result: lbuffer uint8 (size 64) -> Stack bool 
   (requires fun h -> live h b /\ live h result /\ disjoint b result)
-  (ensures fun h0 _ h1 -> modifies (loc result) h0 h1)
+  (ensures fun h0 r h1 -> modifies (loc result) h0 h1 /\
+  	(
+  		let id = Lib.Sequence.index (as_seq h0 b) 0 in 
+  		let x = Lib.Sequence.sub (as_seq h0 b) 1 32 in 
+  			let xResult = Lib.Sequence.sub (as_seq h1 result) 0 32 in 
+  		let y = Lib.Sequence.sub (as_seq h0 b) 33 32 in 
+  			let yResult = Lib.Sequence.sub (as_seq h1 result) 32 32 in 
+  		if uint_v id = 4 then 
+  			r == true /\
+  			x == xResult /\ y == yResult
+  		else 
+  			r == false
+  	)
+)
 
 
 val decompressionCompressedForm: b: compressedForm -> result: lbuffer uint8 (size 64) -> Stack bool 
